src/Config_Morphisms.thy
@@ -43,19 +43,61 @@ fun  morphism_TESL_config
            (\<Gamma>, n \<turnstile> (\<Psi>\<Otimes>f) \<triangleright> (\<Phi>\<Otimes>f))" 
 end
 
-find_theorems name:consistent
+text\<open>A TESL formula is called consistent if it possesses Kripke-models in its denotational 
+interpretation.\<close>
+
+find_theorems TESL_interpretation
 definition consistent :: "('\<tau>::linordered_field) TESL_formula \<Rightarrow> bool" 
   where   "consistent \<Psi> \<equiv> \<lbrakk>\<lbrakk> \<Psi> \<rbrakk>\<rbrakk>\<^sub>T\<^sub>E\<^sub>S\<^sub>L \<noteq> {}"
 
 
+text\<open> For the case of a non-periodic TESL formula, the esta 
+\<close>
+theorem consistency_finite :
+  assumes start             : "([], 0 \<turnstile> \<Psi> \<triangleright> [])  \<hookrightarrow>\<^sup>*\<^sup>* (\<Gamma>\<^sub>1, n\<^sub>1 \<turnstile> [] \<triangleright> [])"
+   and    init_invariant    : "consistent_context \<Gamma>\<^sub>1"
+ shows   "consistent \<Psi>"    
+proof -
+  have * : "\<exists> n. ([], 0 \<turnstile> \<Psi> \<triangleright> []) \<hookrightarrow>\<^bsup>n\<^esup> (\<Gamma>\<^sub>1, n\<^sub>1 \<turnstile> [] \<triangleright> []) "
+    by (simp add: rtranclp_imp_relpowp start)
+  show ?thesis
+  unfolding consistent_context_def consistent_def
+  using "*" consistent_context_def init_invariant soundness by fastforce
+qed
+
+find_theorems name:"sound"
+
+text\<open>For some infinite cases, the idea for a proof scheme looks as follows: if we can derive
+from the initial configuration @{term "([], 0 \<turnstile> \<Psi> \<triangleright> [])"} a start-point of a lasso
+@{term "(\<Gamma>\<^sub>1, n\<^sub>1 \<turnstile> \<Psi>\<^sub>1 \<triangleright> \<Phi>\<^sub>1)"}, and if we can traverse the lasso one time 
+@{term "(\<Gamma>\<^sub>1, n\<^sub>1 \<turnstile> \<Psi>\<^sub>1 \<triangleright> \<Phi>\<^sub>1) \<hookrightarrow>\<^sup>+\<^sup>+ (\<Gamma>\<^sub>2, n\<^sub>2 \<turnstile> \<Psi>\<^sub>2 \<triangleright> \<Phi>\<^sub>2)"} to isomorphic one, 
+we can always always make a derivation along the lasso. If the entry point of the lasso had traces 
+with prefixes consistent to @{term "\<Gamma>\<^sub>1"}, then there exist traces consisting of this prefix and 
+repetitions of the delta-prefix of the lasso which are consistent with @{term "\<Psi>"} which implies
+the logical consistency of  @{term "\<Psi>"}.
+
+So far the idea. Remains to prove it. Why does one symbolic run along a lasso generalises to 
+arbitrary runs ? 
+\<close>
+
 theorem consistency_coinduct : 
-  assumes start             : "([], 0 \<turnstile> \<Psi> \<triangleright> [])  \<hookrightarrow>\<^sup>*\<^sup>* (\<Gamma>\<^sub>1, n\<^sub>1 \<turnstile> \<Psi>\<^sub>1 \<triangleright> \<Phi>\<^sub>1)"
+  assumes start             : "([], 0 \<turnstile> \<Psi> \<triangleright> [])   \<hookrightarrow>\<^sup>*\<^sup>* (\<Gamma>\<^sub>1, n\<^sub>1 \<turnstile> \<Psi>\<^sub>1 \<triangleright> \<Phi>\<^sub>1)"
    and    loop              : "(\<Gamma>\<^sub>1, n\<^sub>1 \<turnstile> \<Psi>\<^sub>1 \<triangleright> \<Phi>\<^sub>1) \<hookrightarrow>\<^sup>+\<^sup>+ (\<Gamma>\<^sub>2, n\<^sub>2 \<turnstile> \<Psi>\<^sub>2 \<triangleright> \<Phi>\<^sub>2)"
    and    init_invariant    : "consistent_context \<Gamma>\<^sub>1"
    and    post_invariant    : "consistent_context \<Gamma>\<^sub>2"
-   and    retract_condition : "(\<Gamma>\<^sub>2, n\<^sub>2 \<turnstile> \<Psi>\<^sub>2 \<triangleright> \<Phi>\<^sub>2) \<Otimes> f = (\<Gamma>\<^sub>2, n\<^sub>2 \<turnstile> \<Psi>\<^sub>1 \<triangleright> \<Phi>\<^sub>1) " 
-  shows   "consistent \<Psi>"    
-   sorry
-
+   and    retract_condition : "(\<Gamma>\<^sub>2, n\<^sub>2 \<turnstile> \<Psi>\<^sub>2 \<triangleright> \<Phi>\<^sub>2) \<Otimes> (f::'\<tau> \<Rightarrow> '\<tau>) = (\<Gamma>\<^sub>2, n\<^sub>2 \<turnstile> \<Psi>\<^sub>1 \<triangleright> \<Phi>\<^sub>1) " 
+  shows   "consistent (\<Psi> :: ('\<tau> :: linordered_field)TESL_formula)"    
+proof -
+  have 1 : "\<exists> n. [], 0 \<turnstile> \<Psi> \<triangleright> [] \<hookrightarrow>\<^bsup>n\<^esup> (\<Gamma>\<^sub>1, n\<^sub>1 \<turnstile> \<Psi>\<^sub>1 \<triangleright> \<Phi>\<^sub>1) "
+    by (meson rtranclp_power start)
+  have 2 : "\<exists> m. (\<Gamma>\<^sub>1, n\<^sub>1 \<turnstile> \<Psi>\<^sub>1 \<triangleright> \<Phi>\<^sub>1) \<hookrightarrow>\<^bsup>m\<^esup> (\<Gamma>\<^sub>2, n\<^sub>2 \<turnstile> \<Psi>\<^sub>2 \<triangleright> \<Phi>\<^sub>2) \<and> m>0"
+    by (meson loop tranclp_power)
+  have 3 : "\<Phi>\<^sub>1 =  \<Phi>\<^sub>2 \<Otimes> f" 
+    using retract_condition by auto
+  have 4 : "\<Psi>\<^sub>1 =  \<Psi>\<^sub>2 \<Otimes> f" 
+    using retract_condition by auto
+  show ?thesis   
+    sorry
+qed
 
 end
